examples/apc/APCTactics.v
@@ -6,21 +6,20 @@ Set Implicit Arguments.
 
 Section APCAUX.
   Import APC.
-  Context {Σ: GRA}.
-  Notation iProp := (iProp Σ).
+  Context `{!invG α Σ Γ, !subG Γ Σ, !sinvG Σ Γ α β τ}.
 
   (* useful apc lemmas - require IST *)
 
   Lemma isim_apc_src
-    contextual fl fr Ist r g {Rs Rt} RR my_tid ps pt nths st_src st_tgt k_src i_tgt spc spc_pure
+    contextual fl fr Ist r g {Rs Rt} RR ps pt nths st_src st_tgt k_src i_tgt u spc spc_pure
     scopes (ow od: Ord.t)
     :
-      (@isim Σ contextual fl fr Ist my_tid r g Rs Rt RR true pt nths
+      (@isim Σ contextual fl fr Ist r g Rs Rt RR true pt nths
         (st_src, k_src ())
         (st_tgt, i_tgt))
     ⊢
-      (@isim Σ contextual fl fr Ist my_tid r g Rs Rt RR ps pt nths 
-        (st_src, ((HMod.sandbox scopes (interp_smod ginv_emp spc (_APC od spc_pure ow))) >>= k_src))
+      (@isim Σ contextual fl fr Ist r g Rs Rt RR ps pt nths 
+        (st_src, ((HMod.sandbox scopes (interp_smod (wsim_ginv u ⊤) spc (_APC od spc_pure ow))) >>= k_src))
         (st_tgt, i_tgt)).
   Proof.
     iIntros "ISIM".
@@ -29,7 +28,7 @@ Section APCAUX.
   Qed.
 
   Lemma isim_apc_tgt
-    contextual fl fr Ist r g {Rs Rt} RR my_tid ps pt nths st_src st_tgt i_src i_tgt spc spc_pure
+    contextual fl fr Ist r g {Rs Rt} RR ps pt nths st_src st_tgt i_src i_tgt u spc spc_pure
     scopes (ow_src ow_tgt od_src od_tgt : Ord.t)
     (WIDTH: (ow_tgt < ow_src)%ord)
     (DEPTH: (od_tgt <= od_src)%ord)
@@ -37,13 +36,13 @@ Section APCAUX.
       ((Ist nths st_src st_tgt) ∗
         (∀ nths0 st_src0 st_tgt0 ow_src_nxt,
           (Ist nths0 st_src0 st_tgt0)
-          -∗ @isim Σ contextual fl fr Ist my_tid r g Rs Rt RR false false nths0
-              (st_src0, ((HMod.sandbox scopes (interp_smod ginv_emp spc (_APC od_src spc_pure ow_src_nxt)));;; i_src))
+          -∗ @isim Σ contextual fl fr Ist r g Rs Rt RR false false nths0
+              (st_src0, ((HMod.sandbox scopes (interp_smod (wsim_ginv u ⊤) spc (_APC od_src spc_pure ow_src_nxt)));;; i_src))
               (st_tgt0, i_tgt)))
     ⊢
-      (@isim Σ contextual fl fr Ist my_tid r g Rs Rt RR ps pt nths 
-        (st_src, ((HMod.sandbox scopes (interp_smod ginv_emp spc (_APC od_src spc_pure ow_src)));;; i_src))
-        (st_tgt, ((HMod.sandbox scopes (interp_smod ginv_emp spc (_APC od_tgt spc_pure ow_tgt)));;; i_tgt))).
+      (@isim Σ contextual fl fr Ist r g Rs Rt RR ps pt nths 
+        (st_src, ((HMod.sandbox scopes (interp_smod (wsim_ginv u ⊤) spc (_APC od_src spc_pure ow_src)));;; i_src))
+        (st_tgt, ((HMod.sandbox scopes (interp_smod (wsim_ginv u ⊤) spc (_APC od_tgt spc_pure ow_tgt)));;; i_tgt))).
   Proof.
     iIntros "[IST ISIM]". iApply isim_reset. iStopProof.
     revert nths st_src. apply combine_quant.
@@ -76,29 +75,29 @@ Section APCAUX.
       steps_l. force_l q4. force_l q5. force_l. iSplitL "GRT"; et.
       call "IST"; iFrame.
       steps_l. forces_r. iSplitL "ASM"; iFrame. steps_r.
-      by_coind "CIH".
+      ITacticsCore.by_coind "CIH".
       iFrame.
     }
     Unshelve. eauto.
   Qed.
 
   Lemma isim_apc_src_call_tgt
-    contextual fl fr Ist r g {Rs Rt} RR my_tid ps pt nths st_src st_tgt k_src k_tgt spc spc_pure
+    contextual fl fr Ist r g {Rs Rt} RR ps pt nths st_src st_tgt k_src k_tgt u spc spc_pure
     scopes fn args fsp (spec_arg: meta fsp) (ow_src ow_fn od_src od_fn : Ord.t)
     (WIDTH: (ow_fn < ow_src)%ord)
     (DEPTH: (od_fn < od_src)%ord)
     (SpcPureInSpc: spc_sub spc_pure spc)
     (fnInSpcPure: spc_pure fn = Some fsp)
     :
-    (((precond fsp my_tid spec_arg od_fn ↑ args) ∗ (Ist nths st_src st_tgt)) ∗
+    (((precond fsp spec_arg od_fn ↑ args) ∗ (Ist nths st_src st_tgt)) ∗
       (∀ nths0 st_src0 st_tgt0 vret ret,
-        (Ist nths0 st_src0 st_tgt0) ∗ (postcond fsp my_tid spec_arg vret ret) 
-        -∗ @isim Σ contextual fl fr Ist my_tid r g Rs Rt RR false false nths0
-            (st_src0, ((HMod.sandbox scopes (interp_smod ginv_emp spc (_APC od_src spc_pure ow_fn))) >>= k_src))
+        (Ist nths0 st_src0 st_tgt0) ∗ (postcond fsp spec_arg vret ret) 
+        -∗ @isim Σ contextual fl fr Ist r g Rs Rt RR false false nths0
+            (st_src0, ((HMod.sandbox scopes (interp_smod (wsim_ginv u ⊤) spc (_APC od_src spc_pure ow_fn))) >>= k_src))
             (st_tgt0, k_tgt ret)))
     ⊢
-      (@isim Σ contextual fl fr Ist my_tid r g Rs Rt RR ps pt nths 
-        (st_src, ((HMod.sandbox scopes (interp_smod ginv_emp spc (_APC od_src spc_pure ow_src))) >>= k_src))
+      (@isim Σ contextual fl fr Ist r g Rs Rt RR ps pt nths 
+        (st_src, ((HMod.sandbox scopes (interp_smod (wsim_ginv u ⊤) spc (_APC od_src spc_pure ow_src))) >>= k_src))
         (st_tgt, (trigger (Call fn args) >>= k_tgt))).
   Proof.
     iIntros "[[PRE IST] ISIM]".
@@ -118,7 +117,7 @@ Section APCAUX.
   Qed.
 
   Lemma isim_apc_src_call_tgt_weaker
-    contextual fl fr Ist r g {Rs Rt} RR my_tid ps pt nths st_src st_tgt k_src k_tgt spc spc_pure
+    contextual fl fr Ist r g {Rs Rt} RR ps pt nths st_src st_tgt k_src k_tgt u spc spc_pure
     scopes fn args fsp' fsp (spec_arg: meta fsp) o P Q (ow_src ow_fn od_src od_fn : Ord.t)
     (WIDTH: (ow_fn < ow_src)%ord)
     (DEPTH: (od_fn < od_src)%ord)
@@ -127,15 +126,15 @@ Section APCAUX.
     (WEAK: fspec_weaker fsp fsp')
     (fspIsfspecapc: fsp = @fspec_apc _ (meta fsp) o (λ x, (P x, Q x)))
     :
-    (((precond fsp my_tid spec_arg od_fn ↑ args) ∗ (Ist nths st_src st_tgt)) ∗
+    (((precond fsp spec_arg od_fn ↑ args) ∗ (Ist nths st_src st_tgt)) ∗
       (∀ nths0 st_src0 st_tgt0 vret ret,
-        (Ist nths0 st_src0 st_tgt0) ∗ (postcond fsp my_tid spec_arg vret ret)
-        -∗ @isim Σ contextual fl fr Ist my_tid r g Rs Rt RR false false nths0
-            (st_src0, ((HMod.sandbox scopes (interp_smod ginv_emp spc (_APC od_src spc_pure ow_fn))) >>= k_src))
+        (Ist nths0 st_src0 st_tgt0) ∗ (postcond fsp spec_arg vret ret)
+        -∗ @isim Σ contextual fl fr Ist r g Rs Rt RR false false nths0
+            (st_src0, ((HMod.sandbox scopes (interp_smod (wsim_ginv u ⊤) spc (_APC od_src spc_pure ow_fn))) >>= k_src))
             (st_tgt0, k_tgt ret)))
     ⊢
-      (@isim Σ contextual fl fr Ist my_tid r g Rs Rt RR ps pt nths
-        (st_src, ((HMod.sandbox scopes (interp_smod ginv_emp spc (_APC od_src spc_pure ow_src))) >>= k_src))
+      (@isim Σ contextual fl fr Ist r g Rs Rt RR ps pt nths
+        (st_src, ((HMod.sandbox scopes (interp_smod (wsim_ginv u ⊤) spc (_APC od_src spc_pure ow_src))) >>= k_src))
         (st_tgt, (trigger (Call fn args) >>= k_tgt))).
   Proof.
     iIntros "[[PRE IST] ISIM]".
@@ -146,7 +145,7 @@ Section APCAUX.
     unfold guarantee. force_l PO. steps_l.
     assert (spc fn = Some fsp'); et. force_l. iSplit; et.
     steps_l.
-    specialize (WEAK my_tid spec_arg). des.
+    specialize (WEAK spec_arg). des.
     force_l x_tgt.
     force_l args.
     iPoseProof ((PRE od_fn ↑ args) with "PRE") as ">PRE".
@@ -160,22 +159,22 @@ Section APCAUX.
   (* useful apc lemmas cont. - don't require IST *)
 
   Lemma isim_apc_tgt_noist
-    contextual fl fr Ist r g {Rs Rt} RR my_tid ps pt nths st_src st_tgt i_src i_tgt
+    contextual fl fr Ist r g {Rs Rt} RR ps pt nths st_src st_tgt i_src i_tgt u
     (spc spc_pure: string → option fspec) (od ow: Ord.t) (scopes: list string)
     (SUB: spc_sub spc_pure spc)
     (SUBA: spc_incl APCA.Spc spc)
-    (FIND: alist_find APCName.apc fr = Some (HMod.sandbox_body (APCA.scopes, interp_sb_hp ginv_emp spc
+    (FIND: alist_find APCName.apc fr = Some (HMod.sandbox_body (APCA.scopes, interp_sb_hp (wsim_ginv u ⊤) spc
         {| fsb_fspec := APCA.apc_spec; fsb_body := cfunN (APCA.apc_body spc_pure) |})))
     (BODY: ∀ fn fsp, spc_pure fn = Some fsp 
-            → ∃ scp, alist_find fn fr = Some (pure_specbody scp spc fsp))
+            → ∃ scopes, alist_find fn fr = Some (pure_specbody scopes u spc fsp))
     :
-      (@isim Σ contextual fl fr Ist my_tid r g Rs Rt RR false false nths
+      (@isim Σ contextual fl fr Ist r g Rs Rt RR false false nths
         (st_src, i_src)
         (st_tgt, i_tgt))
     ⊢
-      (@isim Σ contextual fl fr Ist my_tid r g Rs Rt RR ps pt nths 
+      (@isim Σ contextual fl fr Ist r g Rs Rt RR ps pt nths 
         (st_src, i_src)
-        (st_tgt, ((HMod.sandbox scopes (interp_smod ginv_emp spc (_APC od spc_pure ow)));;; i_tgt))).
+        (st_tgt, ((HMod.sandbox scopes (interp_smod (wsim_ginv u ⊤) spc (_APC od spc_pure ow)));;; i_tgt))).
   Proof.
     iIntros "ISIM".
 
