examples/cellio/MainIAproof.v
@@ -10,12 +10,13 @@ Module MainIA. Section MainIA.
   Definition Ist: nat -> alist key Any.t -> alist key Any.t -> iProp Σ :=
     λ _ st_src st_tgt, emp%I.
 
+  Context (u_s u_t: univ_id).
   Variable Spc: string -> option fspec.
   Hypothesis FooInSpcMap: spc_incl FooAS.Spc Spc.
   Hypothesis InputInSpc: spc_incl InputAS.Spc Spc.
 
-  Local Notation CellioA := (CellioA.t Spc).
-  Local Notation MainA := (MainA.t Spc).
+  Local Notation CellioA := (CellioA.t u_s Spc).
+  Local Notation MainA := (MainA.t u_s Spc).
   Local Notation IstFull := (IstProd (IstSB MainA.(HMod.scopes) Ist) IstEq).
 
   Lemma simF_main:
