theories/simulations/wsim/wsim_tactics.v
@@ -1,67 +1,67 @@
-Require Import CRIS ltac2_lib SchHeader.
+Require Import Common HMod ITactics ltac2_lib.
 Require Export wsim.
 
 From iris.proofmode Require Import coq_tactics environments.
 (* ● ◓ ○ *)
 Notation "E1 '------------------------------------------------------------------□' E2 '------------------------------------------------------------------∗' st_src st_tgt '------------------------------params------------------------------' ○ E r g ps pt '-------------------------------wsim-------------------------------' itr_src itr_tgt" :=
-  (environments.envs_entails (Envs E1 E2 _) (wsim _ _ _ _ None _ _ E r g _ _ _ ps pt _ (st_src, itr_src) (st_tgt, itr_tgt)))
+  (environments.envs_entails (Envs E1 E2 _) (wsim _ _ _ None _ _ E r g _ _ _ ps pt _ (st_src, itr_src) (st_tgt, itr_tgt)))
     (at level 50, only printing,
       format "E1 '------------------------------------------------------------------□' '//' E2 '------------------------------------------------------------------∗' '//' st_src '//' st_tgt '//' '------------------------------params------------------------------' '//' ○ '/' E '/' r '/' g '/' ps '/' pt '//' '-------------------------------wsim-------------------------------' '//' itr_src '//' '//' '//' itr_tgt '//'").
 Notation "E1 '------------------------------------------------------------------□' E2 '------------------------------------------------------------------∗' st_src st_tgt '------------------------------params------------------------------' ◓ E r g ps pt '-------------------------------wsim-------------------------------' itr_src itr_tgt" :=
-  (environments.envs_entails (Envs E1 E2 _) (wsim _ _ _ _ (Some false) _ _ E r g _ _ _ ps pt _ (st_src, itr_src) (st_tgt, itr_tgt)))
+  (environments.envs_entails (Envs E1 E2 _) (wsim _ _ _ (Some false) _ _ E r g _ _ _ ps pt _ (st_src, itr_src) (st_tgt, itr_tgt)))
     (at level 50, only printing,
       format "E1 '------------------------------------------------------------------□' '//' E2 '------------------------------------------------------------------∗' '//' st_src '//' st_tgt '//' '------------------------------params------------------------------' '//' ◓ '/' E '/' r '/' g '/' ps '/' pt '//' '-------------------------------wsim-------------------------------' '//' itr_src '//' '//' '//' itr_tgt '//'").
 Notation "E1 '------------------------------------------------------------------□' E2 '------------------------------------------------------------------∗' st_src st_tgt '------------------------------params------------------------------' ● E r g ps pt '-------------------------------wsim-------------------------------' itr_src itr_tgt" :=
-  (environments.envs_entails (Envs E1 E2 _) (wsim _ _ _ _ (Some true) _ _ E r g _ _ _ ps pt _ (st_src, itr_src) (st_tgt, itr_tgt)))
+  (environments.envs_entails (Envs E1 E2 _) (wsim _ _ _ (Some true) _ _ E r g _ _ _ ps pt _ (st_src, itr_src) (st_tgt, itr_tgt)))
     (at level 50, only printing,
       format "E1 '------------------------------------------------------------------□' '//' E2 '------------------------------------------------------------------∗' '//' st_src '//' st_tgt '//' '------------------------------params------------------------------' '//' ● '/' E '/' r '/' g '/' ps '/' pt '//' '-------------------------------wsim-------------------------------' '//' itr_src '//' '//' '//' itr_tgt '//'").
 Notation "E1 '------------------------------------------------------------------□' st_src st_tgt '------------------------------params------------------------------' ○ E r g ps pt '-------------------------------wsim-------------------------------' itr_src itr_tgt" :=
-  (environments.envs_entails (Envs E1 Enil _) (wsim _ _ _ _ None _ _ E r g _ _ _ ps pt _ (st_src, itr_src) (st_tgt, itr_tgt)))
+  (environments.envs_entails (Envs E1 Enil _) (wsim _ _ _ None _ _ E r g _ _ _ ps pt _ (st_src, itr_src) (st_tgt, itr_tgt)))
     (at level 50, only printing,
       format "E1 '------------------------------------------------------------------□' '//' st_src '//' st_tgt '//' '------------------------------params------------------------------' '//' ○ '/' E '/' r '/' g '/' ps '/' pt '//' '-------------------------------wsim-------------------------------' '//' itr_src '//' '//' '//' itr_tgt '//'").
 Notation "E1 '------------------------------------------------------------------□' st_src st_tgt '------------------------------params------------------------------' ◓ E r g ps pt '-------------------------------wsim-------------------------------' itr_src itr_tgt" :=
-  (environments.envs_entails (Envs E1 Enil _) (wsim _ _ _ _ (Some false) _ _ E r g _ _ _ ps pt _ (st_src, itr_src) (st_tgt, itr_tgt)))
+  (environments.envs_entails (Envs E1 Enil _) (wsim _ _ _ (Some false) _ _ E r g _ _ _ ps pt _ (st_src, itr_src) (st_tgt, itr_tgt)))
     (at level 50, only printing,
       format "E1 '------------------------------------------------------------------□' '//' st_src '//' st_tgt '//' '------------------------------params------------------------------' '//' ◓ '/' E '/' r '/' g '/' ps '/' pt '//' '-------------------------------wsim-------------------------------' '//' itr_src '//' '//' '//' itr_tgt '//'").
 Notation "E1 '------------------------------------------------------------------□' st_src st_tgt '------------------------------params------------------------------' ● E r g ps pt '-------------------------------wsim-------------------------------' itr_src itr_tgt" :=
-  (environments.envs_entails (Envs E1 Enil _) (wsim _ _ _ _ (Some true) _ _ E r g _ _ _ ps pt _ (st_src, itr_src) (st_tgt, itr_tgt)))
+  (environments.envs_entails (Envs E1 Enil _) (wsim _ _ _ (Some true) _ _ E r g _ _ _ ps pt _ (st_src, itr_src) (st_tgt, itr_tgt)))
     (at level 50, only printing,
       format "E1 '------------------------------------------------------------------□' '//' st_src '//' st_tgt '//' '------------------------------params------------------------------' '//' ● '/' E '/' r '/' g '/' ps '/' pt '//' '-------------------------------wsim-------------------------------' '//' itr_src '//' '//' '//' itr_tgt '//'").
 Notation "E2 '------------------------------------------------------------------∗' st_src st_tgt '------------------------------params------------------------------' ○ E r g ps pt '-------------------------------wsim-------------------------------' itr_src itr_tgt" :=
-  (environments.envs_entails (Envs Enil E2 _) (wsim _ _ _ _ None _ _ E r g _ _ _ ps pt _ (st_src, itr_src) (st_tgt, itr_tgt)))
+  (environments.envs_entails (Envs Enil E2 _) (wsim _ _ _ None _ _ E r g _ _ _ ps pt _ (st_src, itr_src) (st_tgt, itr_tgt)))
     (at level 50, only printing,
       format "E2 '------------------------------------------------------------------∗' '//' st_src '//' st_tgt '//' '------------------------------params------------------------------' '//' ○ '/' E '/' r '/' g '/' ps '/' pt '//' '-------------------------------wsim-------------------------------' '//' itr_src '//' '//' '//' itr_tgt '//'").
 Notation "E2 '------------------------------------------------------------------∗' st_src st_tgt '------------------------------params------------------------------' ◓ E r g ps pt '-------------------------------wsim-------------------------------' itr_src itr_tgt" :=
-  (environments.envs_entails (Envs Enil E2 _) (wsim _ _ _ _ (Some false) _ _ E r g _ _ _ ps pt _ (st_src, itr_src) (st_tgt, itr_tgt)))
+  (environments.envs_entails (Envs Enil E2 _) (wsim _ _ _ (Some false) _ _ E r g _ _ _ ps pt _ (st_src, itr_src) (st_tgt, itr_tgt)))
     (at level 50, only printing,
       format "E2 '------------------------------------------------------------------∗' '//' st_src '//' st_tgt '//' '------------------------------params------------------------------' '//' ◓ '/' E '/' r '/' g '/' ps '/' pt '//' '-------------------------------wsim-------------------------------' '//' itr_src '//' '//' '//' itr_tgt '//'").
 Notation "E2 '------------------------------------------------------------------∗' st_src st_tgt '------------------------------params------------------------------' ● E r g ps pt '-------------------------------wsim-------------------------------' itr_src itr_tgt" :=
-  (environments.envs_entails (Envs Enil E2 _) (wsim _ _ _ _ (Some true) _ _ E r g _ _ _ ps pt _ (st_src, itr_src) (st_tgt, itr_tgt)))
+  (environments.envs_entails (Envs Enil E2 _) (wsim _ _ _ (Some true) _ _ E r g _ _ _ ps pt _ (st_src, itr_src) (st_tgt, itr_tgt)))
     (at level 50, only printing,
       format "E2 '------------------------------------------------------------------∗' '//' st_src '//' st_tgt '//' '------------------------------params------------------------------' '//' ● '/' E '/' r '/' g '/' ps '/' pt '//' '-------------------------------wsim-------------------------------' '//' itr_src '//' '//' '//' itr_tgt '//'").
 
 (* additional *) 
 Notation "E1 '------------------------------------------------------------------□' E2 '------------------------------------------------------------------∗' st_src st_tgt '-------------------------------wsim-------------------------------' P '∗' 'WSIM'" :=
-  (environments.envs_entails (Envs E1 E2 _) (bi_sep P (wsim _ _ _ _ _ _ _ _ _ _ _ _ _ _ _ _ _ (st_src, _) (st_tgt, _))))
+  (environments.envs_entails (Envs E1 E2 _) (bi_sep P (wsim _ _ _ _ _ _ _ _ _ _ _ _ _ _ _ _ (st_src, _) (st_tgt, _))))
     (at level 50, only printing,
       format "E1 '------------------------------------------------------------------□' '//' E2 '------------------------------------------------------------------∗' '//' st_src '//' st_tgt '//' '-------------------------------wsim-------------------------------' '//' P  '∗'  'WSIM' ").
 
 Notation "E1 '------------------------------------------------------------------□' E2 '------------------------------------------------------------------∗' st_src st_tgt '-------------------------------wsim-------------------------------' P '-∗' 'WSIM'" :=
-  (environments.envs_entails (Envs E1 E2 _) (bi_wand P (wsim _ _ _ _ _ _ _ _ _ _ _ _ _ _ _ _ _ (st_src, _) (st_tgt, _))))
+  (environments.envs_entails (Envs E1 E2 _) (bi_wand P (wsim _ _ _ _ _ _ _ _ _ _ _ _ _ _ _ _ (st_src, _) (st_tgt, _))))
     (at level 50, only printing,
       format "E1 '------------------------------------------------------------------□' '//' E2 '------------------------------------------------------------------∗' '//' st_src '//' st_tgt '//' '-------------------------------wsim-------------------------------' '//' P  '-∗'  'WSIM' ").
 
 
 Ltac w_replace_l :=
   lazymatch goal with
-  | [ |- environments.envs_entails ?env (wsim ?fl_src ?tl_tgt ?Ist ?my_tid ?t ?u ?v ?E ?r ?g ?R_s ?R_t ?RR ?ps ?pt ?nths (?st_src, ?itr_src) (?st_tgt, ?itr_tgt)) ] =>
-      refine (eq_ind_r (fun itr_src' => environments.envs_entails env (wsim fl_src tl_tgt Ist my_tid t u v E r g R_s R_t RR ps pt nths (st_src, itr_src') (st_tgt, itr_tgt))) _ _); cycle 1
+  | [ |- environments.envs_entails ?env (wsim ?fl_src ?tl_tgt ?Ist ?t ?u ?v ?E ?r ?g ?R_s ?R_t ?RR ?ps ?pt ?nths (?st_src, ?itr_src) (?st_tgt, ?itr_tgt)) ] =>
+      refine (eq_ind_r (fun itr_src' => environments.envs_entails env (wsim fl_src tl_tgt Ist t u v E r g R_s R_t RR ps pt nths (st_src, itr_src') (st_tgt, itr_tgt))) _ _); cycle 1
   end.
 
 Ltac w_replace_r :=
   lazymatch goal with
-  | [ |- environments.envs_entails ?env (wsim ?fl_src ?tl_tgt ?Ist ?my_tid ?t ?u ?v ?E ?r ?g ?R_s ?R_t ?RR ?ps ?pt ?nths (?st_src, ?itr_src) (?st_tgt, ?itr_tgt)) ] =>
-      refine (eq_ind_r (fun itr_tgt' => environments.envs_entails env (wsim fl_src tl_tgt Ist my_tid t u v E r g R_s R_t RR ps pt nths (st_src, itr_src) (st_tgt, itr_tgt'))) _ _); cycle 1
+  | [ |- environments.envs_entails ?env (wsim ?fl_src ?tl_tgt ?Ist ?t ?u ?v ?E ?r ?g ?R_s ?R_t ?RR ?ps ?pt ?nths (?st_src, ?itr_src) (?st_tgt, ?itr_tgt)) ] =>
+      refine (eq_ind_r (fun itr_tgt' => environments.envs_entails env (wsim fl_src tl_tgt Ist t u v E r g R_s R_t RR ps pt nths (st_src, itr_src) (st_tgt, itr_tgt'))) _ _); cycle 1
   end.
 
 Ltac hnorm_itr :=
@@ -101,42 +101,40 @@ Ltac w_hnorm_l := w_replace_l; [s; hnorm_itr|].
 Ltac w_hnorm_r := w_replace_r; [s; hnorm_itr|].
 Ltac _w_step :=
   match goal with
-  | [ |- environments.envs_entails _ (wsim _ _ _ _ _ _ _ _ _ _ _ _ _ _ _ _ (_, Ret _) (_, Ret _))] =>
+  | [ |- environments.envs_entails _ (wsim _ _ _ _ _ _ _ _ _ _ _ _ _ _ _ (_, Ret _) (_, Ret _))] =>
       iApply wsim_ret
-  | [ |- environments.envs_entails _ (wsim _ _ _ _ _ _ _ _ _ _ _ _ _ _ _ _ (_, trigger (IO _ _) >>= _) (_, trigger (IO _ _) >>= _))] =>
+  | [ |- environments.envs_entails _ (wsim _ _ _ _ _ _ _ _ _ _ _ _ _ _ _ (_, trigger (IO _ _) >>= _) (_, trigger (IO _ _) >>= _))] =>
       iApply wsim_io; iIntros "%"
-  | [ |- environments.envs_entails _ (wsim _ _ _ _ _ _ _ _ _ _ _ _ _ _ _ _ (_, trigger (Spawn _ _) >>= _) (_, trigger (Spawn _ _) >>= _))] =>
+  | [ |- environments.envs_entails _ (wsim _ _ _ _ _ _ _ _ _ _ _ _ _ _ _ (_, trigger (Spawn _ _) >>= _) (_, trigger (Spawn _ _) >>= _))] =>
       iApply wsim_spawn
   end.
 
 Ltac _w_step_l :=
   match goal with
-  | [ |- environments.envs_entails _ (wsim _ _ _ _ _ _ _ _ _ _ _ _ _ _ _ _ (_, tau;; _) _) ] =>
+  | [ |- environments.envs_entails _ (wsim _ _ _ _ _ _ _ _ _ _ _ _ _ _ _ (_, tau;; _) _) ] =>
       iApply wsim_tau_src
-  | [ |- environments.envs_entails _ (wsim _ _ _ _ _ _ _ _ _ _ _ _ _ _ _ _ (_, Ret _ >>= _) _) ] =>
+  | [ |- environments.envs_entails _ (wsim _ _ _ _ _ _ _ _ _ _ _ _ _ _ _ (_, Ret _ >>= _) _) ] =>
       rewrite bind_ret_l
-  | [ |- environments.envs_entails _ (wsim _ _ _ _ _ _ _ _ _ _ _ _ _ _ _ _ (_, trigger Tid >>= _) _) ] =>
-      iApply wsim_tid_src
-  | [ |- environments.envs_entails _ (wsim _ _ _ _ _ _ _ _ _ _ _ _ _ _ _ _ (_, trigger (Take _) >>= _) _) ] =>
+  | [ |- environments.envs_entails _ (wsim _ _ _ _ _ _ _ _ _ _ _ _ _ _ _ (_, trigger (Take _) >>= _) _) ] =>
       let name := fresh "q" in iApply wsim_take_src; iIntros (name)
-  | [ |- environments.envs_entails _ (wsim _ _ _ _ _ ?υ _ _ _ _ _ _ _ _ _ _ (_, trigger (Assume ?P) >>= _) _) ] =>
+  | [ |- environments.envs_entails _ (wsim _ _ _ _ ?υ _ _ _ _ _ _ _ _ _ _ (_, trigger (Assume ?P) >>= _) _) ] =>
       first [
         tcsearch constr:(WP P υ ⊤)
           ltac:(fun c =>
-            iApply (wsim_full_assume_src_WP _ _ _ _ _ _ _ _ _ _ _ _ _ _ _ _ _ _ (i:=c)); simpl);
+            iApply (wsim_full_assume_src_WP _ _ _ _ _ _ _ _ _ _ _ _ _ _ _ _ _ (i:=c)); simpl);
         match goal with
         | [ |- environments.envs_entails _ (?P' -∗ _)] =>
           unfold_precond_postcond P'; iIntrosFresh "ASM"
         end
       | unfold_precond_postcond P; iApply wsim_assume_src; iIntrosFresh "ASM"
       ]
-  | [ |- environments.envs_entails _ (wsim _ _ _ _ _ _ _ _ _ _ _ _ _ _ _ _ (_, assume _ >>= _) _) ] =>
+  | [ |- environments.envs_entails _ (wsim _ _ _ _ _ _ _ _ _ _ _ _ _ _ _ (_, assume _ >>= _) _) ] =>
       let name := fresh "asm" in iApply wsim_asm_src; iIntros (name)
-  | [ |- environments.envs_entails _ (wsim _ _ _ _ _ _ _ _ _ _ _ _ _ _ _ _ (_, (HMod.sandbox _ (trigger (SPut _ _))) >>= _) _) ] =>
+  | [ |- environments.envs_entails _ (wsim _ _ _ _ _ _ _ _ _ _ _ _ _ _ _ (_, (HMod.sandbox _ (trigger (SPut _ _))) >>= _) _) ] =>
       iApply wsim_sput_src_sandbox; [s;eauto|]
-  | [ |- environments.envs_entails _ (wsim _ _ _ _ _ _ _ _ _ _ _ _ _ _ _ _ (_, (HMod.sandbox _ (trigger (SGet _))) >>= _) _) ] =>
+  | [ |- environments.envs_entails _ (wsim _ _ _ _ _ _ _ _ _ _ _ _ _ _ _ (_, (HMod.sandbox _ (trigger (SGet _))) >>= _) _) ] =>
       iApply wsim_sget_src_sandbox; [s;eauto|]
-  | [ |- environments.envs_entails _ (wsim _ _ _ _ _ _ _ _ _ _ _ _ _ _ _ _ (_, unwrapU ?ox >>= _) _) ] =>
+  | [ |- environments.envs_entails _ (wsim _ _ _ _ _ _ _ _ _ _ _ _ _ _ _ (_, unwrapU ?ox >>= _) _) ] =>
       let name := fresh "q" in
       iApply wsim_unwrapU_src; iIntros (name) "%";
       match goal with [ H: ?x = Some _ |- _ ] => let G := fresh "G" in rename H into G; try rewrite -> G in * end
@@ -173,37 +171,35 @@ Ltac _w_step_r :=
   match goal with
   (******* isim ******)
   (** tgt **)
-  | [ |- environments.envs_entails _ (wsim _ _ _ _ _ _ _ _ _ _ _ _ _ _ _ _ _ (_, tau;; _)) ] =>
+  | [ |- environments.envs_entails _ (wsim _ _ _ _ _ _ _ _ _ _ _ _ _ _ _ _ (_, tau;; _)) ] =>
       iApply wsim_tau_tgt
-  | [ |- environments.envs_entails _ (wsim _ _ _ _ _ _ _ _ _ _ _ _ _ _ _ _ _ (_, Ret _ >>= _) ) ] =>
+  | [ |- environments.envs_entails _ (wsim _ _ _ _ _ _ _ _ _ _ _ _ _ _ _ _ (_, Ret _ >>= _) ) ] =>
       rewrite bind_ret_l
-  | [ |- environments.envs_entails _ (wsim _ _ _ _ _ _ _ _ _ _ _ _ _ _ _ _ _ (_, trigger (Choose _) >>= _) ) ] =>
+  | [ |- environments.envs_entails _ (wsim _ _ _ _ _ _ _ _ _ _ _ _ _ _ _ _ (_, trigger (Choose _) >>= _) ) ] =>
       let name := fresh "q" in iApply wsim_choose_tgt; iIntros (name)
-  | [ |- environments.envs_entails _ (wsim _ _ _ _ _ _ ?ν _ _ _ _ _ _ _ _ _ _ (_, trigger (Guarantee ?P) >>= _) ) ] =>
+  | [ |- environments.envs_entails _ (wsim _ _ _ _ _ ?ν _ _ _ _ _ _ _ _ _ _ (_, trigger (Guarantee ?P) >>= _) ) ] =>
       first [
         tcsearch constr:(WP P ν ⊤)
           ltac:(fun c =>
-            iApply (wsim_half_guarantee_tgt_WP _ _ _ _ _ _ _ _ _ _ _ _ _ _ _ _ _ _ (i:=c)); simpl);
+            iApply (wsim_half_guarantee_tgt_WP _ _ _ _ _ _ _ _ _ _ _ _ _ _ _ _ _ (i:=c)); simpl);
         match goal with
         | [ |- environments.envs_entails _ (?P' -∗ _)] =>
           unfold_precond_postcond P'; iIntrosFresh "GRT"
         end
       | unfold_precond_postcond P; iApply wsim_guarantee_tgt; iIntrosFresh "GRT"
       ]
-  | [ |- environments.envs_entails _ (wsim _ _ _ _ _ _ _ _ _ _ _ _ _ _ _ _ _ (_, guarantee _ >>= _)) ] =>
+  | [ |- environments.envs_entails _ (wsim _ _ _ _ _ _ _ _ _ _ _ _ _ _ _ _ (_, guarantee _ >>= _)) ] =>
       let name := fresh "grt" in iApply wsim_guar_tgt; iIntros (name)
-  | [ |- environments.envs_entails _ (wsim _ _ _ _ _ _ _ _ _ _ _ _ _ _ _ _ _ (_, (HMod.sandbox _ (trigger (SPut _ _))) >>= _)) ] =>
+  | [ |- environments.envs_entails _ (wsim _ _ _ _ _ _ _ _ _ _ _ _ _ _ _ _ (_, (HMod.sandbox _ (trigger (SPut _ _))) >>= _)) ] =>
       iApply wsim_sput_tgt_sandbox; [s; eauto|]
-  | [ |- environments.envs_entails _ (wsim _ _ _ _ _ _ _ _ _ _ _ _ _ _ _ _ _ (_, (HMod.sandbox _ (trigger (SGet _))) >>= _)) ] =>
+  | [ |- environments.envs_entails _ (wsim _ _ _ _ _ _ _ _ _ _ _ _ _ _ _ _ (_, (HMod.sandbox _ (trigger (SGet _))) >>= _)) ] =>
       iApply wsim_sget_tgt_sandbox; [s; eauto|]
   (* 
-  | [ |- environments.envs_entails _ (isim _ _ _ _ _ _ _ _ _ _ _ _ (_, unwrapN ?ox >>= _)) ] =>
+  | [ |- environments.envs_entails _ (isim _ _ _ _ _ _ _ _ _ _ _ (_, unwrapN ?ox >>= _)) ] =>
       let name := fresh "q" in
       iApply isim_unwrapN_tgt; iIntros (name) "%";
       match goal with [ H: ?x = Some _ |- _ ] => let G := fresh "G" in rename H into G; try rewrite -> G in * end
 *)
-  | [ |- environments.envs_entails _ (wsim _ _ _ _ _ _ _ _ _ _ _ _ _ _ _ _ _ (_, trigger Tid >>= _)) ] =>
-      iApply wsim_tid_tgt
   end.
 
 Ltac w_step_r_core :=
@@ -226,22 +222,22 @@ Ltac w_steps_r :=
 
 Ltac _w_force_l :=
   match goal with
-  | [ |- environments.envs_entails _ (wsim _ _ _ _ _ _ _ _ _ _ _ _ _ _ _ _ (_, trigger (Choose ?T) >>= _) _) ] =>
+  | [ |- environments.envs_entails _ (wsim _ _ _ _ _ _ _ _ _ _ _ _ _ _ _ (_, trigger (Choose ?T) >>= _) _) ] =>
       iApply wsim_choose_src
-  | [ |- environments.envs_entails _ (wsim _ _ _ _ _ ?υ _ _ _ _ _ _ _ _ _ _ (_, trigger (Guarantee ?P) >>= _) _) ] =>
+  | [ |- environments.envs_entails _ (wsim _ _ _ _ ?υ _ _ _ _ _ _ _ _ _ _ (_, trigger (Guarantee ?P) >>= _) _) ] =>
       first [
         tcsearch constr:(WP P υ ⊤)
           ltac:(fun c =>
-            iApply (wsim_full_guarantee_src_WP _ _ _ _ _ _ _ _ _ _ _ _ _ _ _ _ _ _ (i:=c)); simpl);
+            iApply (wsim_full_guarantee_src_WP _ _ _ _ _ _ _ _ _ _ _ _ _ _ _ _ _ (i:=c)); simpl);
         match goal with
         | [ |- environments.envs_entails _ (?P' ∗ _)] =>
           unfold_precond_postcond P'
         end
       | unfold_precond_postcond P; iApply wsim_guarantee_src
       ]
-  | [ |- environments.envs_entails _ (wsim _ _ _ _ _ _ _ _ _ _ _ _ _ _ _ _ (_, unwrapN _ >>= _) _) ] =>
+  | [ |- environments.envs_entails _ (wsim _ _ _ _ _ _ _ _ _ _ _ _ _ _ _ (_, unwrapN _ >>= _) _) ] =>
       iApply wsim_unwrapN_src
-  (* | [ |- environments.envs_entails _ (isim _ _ _ _ _ _ _ _ _ _ _ (_, guarantee _ >>= _) _) ] =>
+  (* | [ |- environments.envs_entails _ (isim _ _ _ _ _ _ _ _ _ _ (_, guarantee _ >>= _) _) ] =>
       iApply isim_guar_src *)
   end.
 
@@ -264,22 +260,22 @@ Ltac w_forces_l :=
 
 Ltac _w_force_r :=
   match goal with
-  | [ |- environments.envs_entails _ (wsim _ _ _ _ _ _ _ _ _ _ _ _ _ _ _ _ _ (_, trigger (Take _) >>= _)) ] =>
+  | [ |- environments.envs_entails _ (wsim _ _ _ _ _ _ _ _ _ _ _ _ _ _ _ _ (_, trigger (Take _) >>= _)) ] =>
       iApply wsim_take_tgt
-  | [ |- environments.envs_entails _ (wsim _ _ _ _ _ _ ?ν _ _ _ _ _ _ _ _ _ _ (_, trigger (Assume ?P) >>= _)) ] =>
+  | [ |- environments.envs_entails _ (wsim _ _ _ _ _ ?ν _ _ _ _ _ _ _ _ _ _ (_, trigger (Assume ?P) >>= _)) ] =>
       first [
         tcsearch constr:(WP P ν ⊤)
           ltac:(fun c =>
-            iApply (wsim_half_assume_tgt_WP _ _ _ _ _ _ _ _ _ _ _ _ _ _ _ _ _ _ (i:=c)); simpl);
+            iApply (wsim_half_assume_tgt_WP _ _ _ _ _ _ _ _ _ _ _ _ _ _ _ _ _ (i:=c)); simpl);
         match goal with
         | [ |- environments.envs_entails _ (?P' ∗ _)] =>
           unfold_precond_postcond P'
         end
       | unfold_precond_postcond P; iApply wsim_assume_tgt
       ]
-  | [ |- environments.envs_entails _ (wsim _ _ _ _ _ _ _ _ _ _ _ _ _ _ _ _ _ (_, assume _ >>= _)) ] =>
+  | [ |- environments.envs_entails _ (wsim _ _ _ _ _ _ _ _ _ _ _ _ _ _ _ _ (_, assume _ >>= _)) ] =>
       iApply wsim_asm_tgt
-  (* | [ |- environments.envs_entails _ (isim _ _ _ _ _ _ _ _ _ _ _ _ (_, unwrapU _ >>= _)) ] =>
+  (* | [ |- environments.envs_entails _ (isim _ _ _ _ _ _ _ _ _ _ _ (_, unwrapU _ >>= _)) ] =>
       iApply isim_unwrapU_tgt; iExists _ *)
   end
 .
@@ -357,7 +353,7 @@ Ltac init_simF :=
   step_l.
 
 Ltac init_wsim u_src u_tgt :=
-  init_simF; iApply (wsim_init _ _ _ _ u_src u_tgt).
+  init_simF; iApply (wsim_init _ _ _ u_src u_tgt).
 
 Ltac unfold_iter_l :=
   let marker := fresh "MARKER" in
